src/refinement/PromisingPF_AlgorithmicPF.v
@@ -23,6 +23,32 @@ Require Import CertifyFacts.
 
 Set Implicit Arguments.
 
+Lemma amachine_step_backward
+      m1 m2 tlocks2
+      (STEP: Machine.step ExecUnit.promise_step m1 m2)
+      (WF1: Machine.wf m1)
+      (WF2: AMachine.wf (AMachine.mk m2 tlocks2)):
+  exists tlocks1,
+    <<STEP: AMachine.step ExecUnit.promise_step (AMachine.mk m1 tlocks1) (AMachine.mk m2 tlocks2)>> /\
+    <<WF: AMachine.wf (AMachine.mk m1 tlocks1)>>.
+Proof.
+Admitted.
+
+Lemma amachine_rtc_step_backward
+      m1 m2 tlocks2
+      (STEP: rtc (Machine.step ExecUnit.promise_step) m1 m2)
+      (WF1: Machine.wf m1)
+      (WF2: AMachine.wf (AMachine.mk m2 tlocks2)):
+  exists tlocks1,
+    <<STEP: rtc (AMachine.step ExecUnit.promise_step) (AMachine.mk m1 tlocks1) (AMachine.mk m2 tlocks2)>> /\
+    <<WF: AMachine.wf (AMachine.mk m1 tlocks1)>>.
+Proof.
+  revert WF1. induction STEP; eauto. i. exploit IHSTEP; eauto.
+  { eapply Machine.step_promise_step_wf; eauto. }
+  i. des.
+  exploit amachine_step_backward; eauto. i. des.
+  esplits; eauto.
+Qed.
 
 Theorem promising_pf_to_algorithmic_pf
         p m
@@ -31,10 +57,25 @@ Theorem promising_pf_to_algorithmic_pf
 Proof.
   inv EXEC. econs; ss.
   - instantiate (1 := AMachine.mk m1 (fun tid => option_map (fun _ => Lock.init) (IdMap.find tid m1.(Machine.tpool)))).
-    (* TODO
-     - rtc_state_step_certify_bot : lock.init at last
-     - one step from the end..
-     *)
-    admit.
+    exploit amachine_rtc_step_backward; eauto.
+    { apply Machine.init_wf. }
+    { instantiate (1 := (fun tid => option_map (fun _ => Lock.init) (IdMap.find tid m1.(Machine.tpool)))).
+      econs; ss.
+      - eapply Machine.rtc_step_promise_step_wf; eauto.
+        apply Machine.init_wf.
+      - i. inv STEP2. specialize (TPOOL tid). inv TPOOL; ss.
+        exploit rtc_state_step_certify_bot; eauto. ss.
+        destruct b. ss. eapply NOPROMISE. eauto.
+      - apply AMachine.init_tlocks_consistent.
+    }
+    i. des.
+    assert (tlocks1 = (fun tid => option_map (fun _ => Lock.init) (IdMap.find tid p))).
+    { inv WF. ss. funext. i. specialize (CERTIFY x). revert CERTIFY.
+      rewrite IdMap.map_spec. destruct (IdMap.find x p); ss.
+      - i. inv CERTIFY. apply no_promise_certify_inv in REL; ss. congr.
+      - i. inv CERTIFY. ss.
+    }
+    subst. apply STEP.
   - ss.
-Admitted.
+  - s. i. destruct (IdMap.find tid (Machine.tpool m1)); ss. inv FIND. ss.
+Qed.
